theories/example.v
@@ -1,0 +1,42 @@
+(** * Examples *)
+Module Example.
+
+Axiom ℕ : atom.
+Axiom pred : atom.
+Example nat_example := [{
+  data ℕ := 𝟙 + ℕ;
+  def pred : Π:ℕ, ℕ := \:ℕ => case unfold<ℕ> 0 of 1 | 0
+}].
+
+End Example.
+
+(* TODO: explain the unconventional definition of [ectx]. *)
+
+(* BD: Something seems off with this definition of evaluation
+   contexts, as there are no inductive occurences of ectx.
+
+   How to construct the context (v1, (v2, [ ]) ), for example?
+ *)
+
+Definition ex_ctx (e1 : expr) : expr :=
+  <{ ((), ( (), e1) ) }> .
+
+Example ex_ctx_bad : ~ ectx ex_ctx.
+Proof.
+  unfold ex_ctx; intro H; inversion H; subst;
+    try (generalize (f_equal_help _ _ _ _ H1 (eq_refl (ELit true))); intro; discriminate);
+    try (generalize (f_equal_help _ _ _ _ H0 (eq_refl (ELit true))); intro; discriminate).
+Qed.
+
+(* BD: Turn out that non-recursive contexts aren't a problem, since
+   [SCTx] can be applied recursively. *)
+Example ex_ctx_stuck :
+  forall Σ, Σ ⊨ (ex_ctx <{if true then true else false}>) -->! <{( (), ( (), true) )}>.
+Proof.
+  intros; unfold ex_ctx; eauto.
+  eapply SCtx with (ℇ := fun e => <{( (), e)}> );
+    [repeat econstructor| ].
+  eapply SCtx with (ℇ := fun e => <{( (), e)}> );
+    [repeat econstructor| ].
+  econstructor.
+Qed.
